working on LF of uniform sampling

proof/rejection_sampling/UniformSampling_Concrete_LF.ec
@@ -21,6 +21,7 @@ axiom sub_g_comp_2 x : 1 < x => sub_g x = sub_step (x-1) ++ sub_g (x - 1).
 
 op sub_f (x : int) : leakages_t = sub_g x ++ sub_prefix.
 
+
 lemma bn_subc_leakages start_l :
    hoare [ M(Syscall).bn_subc : M.leakages = start_l ==> M.leakages = sub_f 32 ++ start_l ].
 proof. 
@@ -62,7 +63,6 @@ qed.
 
 
 
-
 (* set0 LEAKAGES  *)
 op set0_prefix : leakages_t = LeakFor (0, 32) :: LeakAddr [] :: [].
 op set0_step (i : int) : leakages_t = LeakAddr [i] :: LeakAddr [] :: [].
@@ -91,23 +91,22 @@ qed.
 
 (* SAMPLING LEAKAGES  *)
 op samp_prefix : leakages_t = 
-  LeakCond true :: LeakAddr [] :: LeakAddr [] :: LeakAddr [] :: LeakAddr [] :: 
-   LeakAddr [] :: (set0_f 32 ++ [LeakAddr []]).
-
+  LeakCond (! set0_64_.`2) :: LeakAddr [] :: LeakAddr [] :: (set0_f 32 ++
+                                                           [LeakAddr [];
+                                                              LeakAddr []]).
 op samp_g (x : int) : leakages_t.
-op samp_step (i : int) : leakages_t = LeakCond true :: LeakAddr [] :: LeakAddr [] :: LeakAddr [] :: LeakAddr [] :: (
-sub_f 32 ++
-LeakAddr [] :: (copy_f 32 ++
-                LeakAddr [] :: LeakAddr [] :: [])) .
-
-  
+op samp_step (i : int) : leakages_t = LeakCond true :: LeakAddr [] :: LeakAddr [] :: (sub_f 32 ++
+                                                LeakAddr [] :: (copy_f 32 ++
+                                                                LeakAddr [] :: 
+                                                                LeakAddr [] :: [])) .
+ 
 
 axiom samp_g_comp_1 x : 0 <= x  => samp_g x = [].
 axiom samp_g_comp_2 x : 0 < x => samp_g x = samp_step (x-1) ++ samp_g (x - 1).
 
 
 op samp_suffix : leakages_t = 
- LeakCond false :: LeakAddr [] :: LeakAddr [] :: LeakAddr [] :: LeakAddr [] :: (
+ LeakCond false :: LeakAddr [] :: LeakAddr []  :: (
 sub_f 32 ++
 LeakAddr [] :: (copy_f 32 ++ LeakAddr [] :: LeakAddr [] :: [])).
 
@@ -122,19 +121,20 @@ lemma rsample_leakages :
    hoare [ M(Syscall).rsample : M.leakages = [] ==> M.leakages = samp_t res.`1].
 proc.
 seq 17 :  (M.leakages = samp_prefix /\ i = 0  /\ cf = false ).
-wp. ecall (bn_set0_leakages M.leakages). wp. skip. progress.  admit. rewrite /set0_64. simplify.
-
+wp. ecall (bn_set0_leakages M.leakages). wp. skip. progress.  
+rewrite /set0_64. simplify.
 while (0 <= i /\ (cf = false => M.leakages = samp_f i) 
               /\ (cf = true => M.leakages = samp_t i)).
-wp. 
-ecall (bn_subc_leakages M.leakages). wp. ecall (bn_copy_leakages M.leakages). wp.  inline*. wp. rnd. wp.  skip. progress.
-smt().  rewrite H4.  rewrite H0. rewrite H2. auto.
+wp.  ecall (bn_subc_leakages M.leakages). simplify.
+wp.  ecall (bn_copy_leakages M.leakages). simplify.
+wp. inline Syscall.randombytes_256. wp. rnd.  wp.
+skip. progress. smt().  rewrite H4.  rewrite H0. rewrite H2. auto. simplify.
 rewrite /samp_f. rewrite (samp_g_comp_2 (i{hr} + 1)). smt().
 simplify.
- rewrite /samp_step.   
-admit.  rewrite H4. rewrite H0. rewrite H2. auto.
+rewrite /samp_step. simplify. smt(@List).
 rewrite /samp_t. simplify.
-rewrite /samp_suffix. admit.
+rewrite /samp_suffix.  simplify.  split. rewrite H4. auto.
+rewrite H0. rewrite H2. auto. smt(@List).
 skip. progress. rewrite /samp_prefix. rewrite /samp_f. rewrite samp_g_comp_1.
 auto. rewrite /samp_prefix. auto.
 rewrite H2. rewrite H. auto.
@@ -144,7 +144,7 @@ qed.
 
 require import W64_SchnorrExtract.
 module M1 = W64_SchnorrExtract_ct.M(W64_SchnorrExtract_ct.Syscall).
-module M2 = W64_SchnorrExtract.M(W64_SchnorrExtract.Syscall).  (* Ring_ops_extract.M(Ring_ops_extract.Syscall). *)
+module M2 = W64_SchnorrExtract.M(W64_SchnorrExtract.Syscall).  
 
 lemma aaaa :
   equiv  [ M1.bn_set0 ~ M2.bn_set0 
@@ -162,6 +162,8 @@ require import Ring_ops_proof.
 require import Ring_ops_spec.
 require import UniformSampling_Abstract.
 require import UniformSampling_Concrete.
+
+
 
 equiv rsample_cspec2:
  M1.rsample ~ CSpecFp.rsample:
@@ -188,6 +190,22 @@ conseq rsample_cspec2. progress. progress. smt().
 qed.
 
 
+lemma sameww a &m : 
+  Pr[ M1.rsample(a) @ &m : true  ] = if 0%r < mu D (RSP (valR a)) then 1%r else 0%r.
+case (0%r < mu D (RSP (valR a))). move => pos. 
+rewrite - (rsample_lossless (W64xN.valR a) &m _). auto. 
+byequiv.
+conseq rsample_cspec2. progress. progress. smt().
+move => neg.
+have -> : Pr[M1.rsample(a) @ &m : true] = Pr[CSpecFp.rsample(W64xN.valR a) @ &m : true].
+byequiv. conseq rsample_cspec2. auto. auto. auto.
+print rsample_lossless0.
+apply (rsample_lossless0 (W64xN.valR a) &m (fun _ => true)).  smt().
+qed.
+
+
+
+
 lemma zzz a i x &m : 
   Pr[ M1.rsample(a) @ &m : res = (i,x)  ]
    =   Pr[ CSpecFp.rsample(W64xN.valR a) @ &m : res = (i, W64xN.valR x)  ].
@@ -204,12 +222,12 @@ hoare. simplify.
 conseq rsample_leakages. auto. auto. auto.
 qed.
 
-lemma qq a l x &m : (glob M1){m} = [] => 0%r < mu D (RSP (valR a)) =>
+lemma qq a l x &m : (glob M1){m} = [] => 
   Pr[ M1.rsample(a) @ &m : M1.leakages = l  /\ res.`2 = x ]
   = Pr[ M1.rsample(a) @ &m : l = samp_t res.`1 /\ res.`2 = x  ].
-move => m1p m2p.
-have pr1 :  Pr[ M1.rsample(a) @ &m : M1.leakages = samp_t res.`1   ] = 1%r.
-rewrite - (samew a &m).   auto.
+move => m1p.
+have pr1 :  Pr[ M1.rsample(a) @ &m : M1.leakages = samp_t res.`1   ] = b2r (0%r < mu D (RSP (valR a))).
+rewrite - (sameww a &m).   auto.
   have ->: Pr[M1.rsample(a) @ &m : true] 
    = Pr[M1.rsample(a) @ &m : M1.leakages = samp_t res.`1 ] + Pr[M1.rsample(a) @ &m : M1.leakages <> samp_t res.`1  ]. rewrite Pr[mu_split (M1.leakages = samp_t res.`1) ]. simplify. auto. rewrite (qq' a &m). auto.
 simplify. auto.
@@ -235,13 +253,11 @@ qed.
 require import AuxLemmas.
 
 
-
-
     
-lemma qqq a x l &m : (glob M1){m} = [] => 0%r < mu D (RSP (valR a)) =>
+lemma qqq a x l &m : (glob M1){m} = [] => (* 0%r < mu D (RSP (valR a)) => *)
   Pr[ M1.rsample(a) @ &m : M1.leakages = l  /\ res.`2 = x  ]
   = Pr[ M1.rsample(a) @ &m :  (inv (-1) samp_t) l = res.`1  /\ res.`2 = x  ].
-move => ic ic'. rewrite  (qq a  l x &m). auto. auto.
+move => ic (* ic' *). rewrite  (qq a  l x &m). auto. auto.
 simplify. 
 have -> : 
   Pr[M1.rsample(a) @ &m :
@@ -283,7 +299,6 @@ qed.
 
 
 
-
 lemma ph_l5''_var &m a : Pr[M1.rsample(a) @ &m : res.`1 <= 0 ] = 0%r.
 byphoare (_: arg = a ==> _);auto. hoare.
 proc.  simplify.
@@ -300,12 +315,13 @@ qed.
 
 
 op g a x l : real 
- = if inv (-1) samp_t l <= 0 then 0%r else mu D (predC (RSP ((valR a)))) ^ (inv (-1) samp_t l - 1) *
-        (mu1 D ((valR x))).
+ = if inv (-1) samp_t l <= 0 \/ valR a <= valR x then 0%r else 
+     mu D (predC (RSP (valR a))) ^ (inv (-1) samp_t l - 1)
+       * (mu1 D (valR x)).
 
         
-lemma leakfree &m x a l: (glob M1){m} = [] => valR x < valR a => 0%r < mu D (RSP (valR a)) =>
-  Pr[ M1.rsample(a) @ &m : M1.leakages = l  /\ res.`2 = x  ]
+lemma leakfree1 &m x a l: (glob M1){m} = [] 
+  => Pr[ M1.rsample(a) @ &m : M1.leakages = l  /\ res.`2 = x  ]
     = g a x l.
       progress.
    rewrite  (qqq a x l &m);auto.
@@ -321,8 +337,21 @@ have -> :
    inv (-1) samp_t l = res.`1 /\ res.`2 = x]
   = Pr[M1.rsample(a) @ &m :
    res = (inv (-1) samp_t l , x) ]. rewrite Pr[mu_eq]. smt(). auto.
+case (valR x < valR a) => case1.
 rewrite zzz.
 rewrite rsample_pr.   smt().
 rewrite /RSP. auto.
 rewrite /z. smt().
+rewrite /g. 
+have ->: (valR a <= valR x) = true. smt(). simplify.
+have : Pr[W64_SchnorrExtract_ct.M(W64_SchnorrExtract_ct.Syscall).rsample(a) @ &m :
+   res.`2 = x] = 0%r.
+  have -> : Pr[W64_SchnorrExtract_ct.M(W64_SchnorrExtract_ct.Syscall).rsample(a) @ &m :
+     res.`2 =  x] = Pr[ CSpecFp.rsample(W64xN.valR a) @ &m : res.`2 =  W64xN.valR x ].
+  byequiv. conseq rsample_cspec2. auto. progress. rewrite H0.  auto.  smt(@W64xN). auto. auto.
+  apply rsample_pr_out. auto.
+smt(@Distr).
+qed.
+
+
 qed.
